SModTr redefined with removed mask parameter

theories/modules/SModTr.v
@@ -1,7 +1,7 @@
-Require Import Mod FSpec Sp.
 Require Import Common ConcRA.
+Require Import Mod FSpec Sp.
 
-Definition mask {Σ : GRA} : Type := ∀ X, crisE X → bool.
+(* Definition mask {Σ : GRA} : Type := ∀ X, crisE X → bool.
 
 Definition mask_handle `{Σ : GRA, E -< crisE} (msk : mask) {T} (e : E T) : itreeV crisE T :=
   if msk T (subevent _ e)
@@ -13,62 +13,62 @@ Definition mask_trigger `{Σ : GRA, E -< crisE} (msk : mask) {X} (e : E X) : itr
 
 Lemma mask_trigger_gen `{Σ : GRA, E -< crisE} (msk : mask) {X} (e : E X) :
   mask_trigger msk e = if msk X (subevent _ e) then trigger e else triggerUB.
-Proof. rewrite /mask_trigger /mask_handle; des_if; rewrite ?bind_ret_r /triggerUB //=; grind. Qed.
+Proof. rewrite /mask_trigger /mask_handle; des_if; rewrite ?bind_ret_r /triggerUB //=; grind. Qed. *)
 
 (* function semantics *)
-Definition fnsem `{Σ : GRA} : Type :=
-  mask *          (* event masks *)
-  option fspec *  (* function spec *)
-  fbody.          (* function body *)
+(* Definition fnsem `{Σ : GRA} : Type :=
+  mask *        
+  option fspec *
+  fbody.         *)
 
 Module SModTr. Section HOARE.
   Context `{!crisG Γ Σ α β τ _S _I, !concG}.
   Implicit Types (fn : string) (varg arg : Any.t) (fspo sspo : option fspec).
-  Implicit Types (msk : mask).
+  (* Implicit Types (msk : mask). *)
   Implicit Types (N : namespace) (stid ntid : nat) (sp : sp_type).
 
   (* Wraps a function call into a Hoare triple *)
-  Definition HoareCall msk fspo fn varg N stid : itree crisE Any.t :=
+  Definition HoareCall fspo fn varg N stid : itree crisE Any.t :=
     match fspo with
     | Some fsp =>
-        x <- mask_trigger msk (Choose (meta fsp));;
+        x <- trigger (Choose (meta fsp));;
 
         (* precondition and argument passing *)
-        arg <- mask_trigger msk (Choose Any.t);;
-        mask_trigger msk (Guarantee (TID stid ∗ YIELD stid ∗ winv (↑N, ↑N)));;;
-        mask_trigger msk (Guarantee ((precond fsp) (N, stid) x varg arg));;;
+        arg <- trigger (Choose Any.t);;
+        trigger (Guarantee (TID stid ∗ YIELD stid ∗ winv (↑N, ↑N)));;;
+        trigger (Guarantee ((precond fsp) (N, stid) x varg arg));;;
 
         (* call *)
-        ret <- mask_trigger msk (Call fn arg);;
+        ret <- trigger (Call fn arg);;
 
-        (* postcondition argument receiving *)
-        vret <- mask_trigger msk (Take Any.t);;
-        mask_trigger msk (Assume (TID stid ∗ YIELD stid ∗ winv (↑N, ↑N)));;;
-        mask_trigger msk (Assume ((postcond fsp) (N, stid) x vret ret));;;
+        (* postcondition and argument receiving *)
+        vret <- trigger (Take Any.t);;
+        trigger (Assume (TID stid ∗ YIELD stid ∗ winv (↑N, ↑N)));;;
+        trigger (Assume ((postcond fsp) (N, stid) x vret ret));;;
         Ret vret
     | None =>
-        mask_trigger msk (Call fn varg)
+        trigger (Call fn varg)
     end.
 
   (* Wraps a function into a Hoare triple *)
   Definition HoareFun
-      msk fspo (body : namespace → nat → Any.t → itree crisE Any.t) : Any.t → itree crisE Any.t :=
+      fspo (body : namespace → nat → Any.t → itree crisE Any.t) : Any.t → itree crisE Any.t :=
     match fspo with
     | Some fsp => λ arg,
-        '(N, stid) : _ <- mask_trigger msk (Take (namespace * nat));;
+        '(N, stid) : _ <- trigger (Take (namespace * nat));;
 
         (* precondition *)
-        x <- mask_trigger msk (Take (meta fsp));;
-        varg <- mask_trigger msk (Take Any.t);;
-        mask_trigger msk (Assume (TID stid ∗ YIELD stid ∗ winv (↑N, ↑N)));;;
-        mask_trigger msk (Assume (precond fsp (N, stid) x varg arg));;;
+        x <- trigger (Take (meta fsp));;
+        varg <- trigger (Take Any.t);;
+        trigger (Assume (TID stid ∗ YIELD stid ∗ winv (↑N, ↑N)));;;
+        trigger (Assume (precond fsp (N, stid) x varg arg));;;
 
         vret <- body N stid varg;;
 
         (* postcondition *)
-        ret <- mask_trigger msk (Choose Any.t);;
-        mask_trigger msk (Guarantee (TID stid ∗ YIELD stid ∗ winv (↑N, ↑N)));;;
-        mask_trigger msk (Guarantee (postcond fsp (N, stid) x vret ret));;;
+        ret <- trigger (Choose Any.t);;
+        trigger (Guarantee (TID stid ∗ YIELD stid ∗ winv (↑N, ↑N)));;;
+        trigger (Guarantee (postcond fsp (N, stid) x vret ret));;;
 
         Ret ret
     | None => λ arg, tau;; body nroot 0 arg
@@ -78,49 +78,49 @@ Module SModTr. Section HOARE.
     trigger (Spawn fn arg). *)
 
   (* Wraps a spawn into a Hoare triple *)
-  Definition HoareSpawn msk fspo sspo fn varg N : itree crisE nat :=
+  Definition HoareSpawn fspo sspo fn varg N : itree crisE nat :=
     match fspo, sspo with
     | Some fsp, Some _ =>
-        x <- mask_trigger msk (Choose (meta fsp));;
-        arg <- mask_trigger msk (Choose Any.t);;
-        tid <- mask_trigger msk (Spawn fn arg);;
-        mask_trigger msk (Assume (YIELD tid));;;
-        mask_trigger msk (Guarantee (precond fsp (N, tid) x varg arg));;;
+        x <- trigger (Choose (meta fsp));;
+        arg <- trigger (Choose Any.t);;
+        tid <- trigger (Spawn fn arg);;
+        trigger (Assume (YIELD tid));;;
+        trigger (Guarantee (precond fsp (N, tid) x varg arg));;;
         Ret tid
     | None, Some _ =>
-        tid <- mask_trigger msk (Spawn fn varg);;
-        mask_trigger msk (Assume (YIELD tid));;;
+        tid <- trigger (Spawn fn varg);;
+        trigger (Assume (YIELD tid));;;
         Ret tid
     | _, None =>
-        mask_trigger msk (Spawn fn varg)
+        trigger (Spawn fn varg)
     end.
 
   (* Definition NativeYield (tid : nat) : itree crisE unit :=
     trigger (Yield tid). *)
 
   (* Wraps a yield into a Hoare triple *)
-  Definition HoareYield msk sspo N stid ntid : itree crisE unit :=
+  Definition HoareYield sspo N stid ntid : itree crisE unit :=
     match sspo with
     | Some _ =>
-      mask_trigger msk (Guarantee (TID stid ∗ YIELD ntid ∗ winv (↑N, ↑N)));;;
-      mask_trigger msk (Yield ntid);;;
-      mask_trigger msk (Assume (TID stid ∗ YIELD stid ∗ winv (↑N, ↑N)))
+      trigger (Guarantee (TID stid ∗ YIELD ntid ∗ winv (↑N, ↑N)));;;
+      trigger (Yield ntid);;;
+      trigger (Assume (TID stid ∗ YIELD stid ∗ winv (↑N, ↑N)))
     | None =>
-      mask_trigger msk (Yield ntid)
+      trigger (Yield ntid)
     end.
 
   (* Definition NativeGetTid : itree crisE nat :=
     trigger GetTid. *)
 
-  Definition HoareGetTid msk sspo stid : itree crisE nat :=
+  Definition HoareGetTid sspo stid : itree crisE nat :=
     match sspo with
     | Some _ =>
-      mask_trigger msk (Guarantee (TID(stid)));;;
-      tid <- mask_trigger msk GetTid;;
-      mask_trigger msk (Assume (⌜tid = stid⌝ ∗ TID(stid)));;;
+      trigger (Guarantee (TID(stid)));;;
+      tid <- trigger GetTid;;
+      trigger (Assume (⌜tid = stid⌝ ∗ TID(stid)));;;
       Ret tid
     | None =>
-      mask_trigger msk GetTid
+      trigger GetTid
     end.
 
   (* Definition handle (img : bool) (sp : sp_type) : crisE ~> itreeV crisE.
@@ -142,202 +142,165 @@ Module SModTr. Section HOARE.
     { exact (inr (existT _ (subevent _ p, λ v, Ret v))). }
     { exact (inr (existT _ (subevent _ c, λ v, Ret v))). }
   Defined. *)
-  Definition handle sp msk N stid : crisE ~> itreeV crisE.
+  Definition handle sp N stid : crisE ~> itreeV crisE.
   Proof.
     intros T e.
     destruct e as [e|e].
     { (* agE *)
-      exact (mask_handle msk e).
+      exact (inr (existT _ (subevent _ e, λ v, Ret v))).
     }
     destruct e as [[fn args|fn args|tid|]|e].
     { (* Call *)
-      exact (inl (HoareCall msk (sp (speckey_fn fn)) fn args N stid)).
+      exact (inl (HoareCall (sp (speckey_fn fn)) fn args N stid)).
     }
     { (* Spawn *)
-      exact (inl (HoareSpawn msk (sp (speckey_fn fn)) (sp (speckey_concE)) fn args N)).
+      exact (inl (HoareSpawn (sp (speckey_fn fn)) (sp (speckey_concE)) fn args N)).
     }
     { (* Yield *)
-      exact (inl (HoareYield msk (sp (speckey_concE)) N stid tid)).
+      exact (inl (HoareYield (sp (speckey_concE)) N stid tid)).
     }
     { (* GetTid *)
-      exact (inl (HoareGetTid msk (sp (speckey_concE)) stid)).
+      exact (inl (HoareGetTid (sp (speckey_concE)) stid)).
     }
     (* pgE +' coreE *)
-    destruct e as [e|e]; exact (mask_handle msk e).
+    destruct e as [e|e]; exact (inr (existT _ (subevent _ e, λ v, Ret v))).
   Defined.
 
   (* Definition trans img sp {R} (it : itree crisE R) : itree crisE R :=
     interpV (handle img sp) it. *)
-  Definition trans sp msk N stid {R} (itr : itree crisE R) : itree crisE R :=
-    interpV (handle sp msk N stid) itr.
+  Definition trans sp N stid {R} (itr : itree crisE R) : itree crisE R :=
+    interpV (handle sp N stid) itr.
   (* Definition trans_body : (bool * sp_type * option fspec) → fbody → fbody :=
     λ '(img, sp, fsp) bd, HoareFun fsp (trans img sp ∘ bd). *)
 
   (* Definition trans_ktree sp (sb : fnsem_type (option fspec * fbody)) : fnsem_type fbody :=
     map_snd (λ '(fsp,bd), trans_body (is_some sb.2.1, if sb.1.1.1 then sp else sp_none, fsp) bd) sb. *)
-  Definition trans_fnsem (sp : sp_type) (sem : fnsem) : fbody :=
-    let '(msk, fspo, fbd) := sem in
-    HoareFun msk fspo (λ N stid, trans sp msk N stid ∘ fbd).
+  Definition trans_fnsem (sp : sp_type) (sem : option fspec * fbody) : fbody :=
+    let '(fspo, fbd) := sem in
+    HoareFun fspo (λ N stid, trans sp N stid ∘ fbd).
 End HOARE. End SModTr.
 
 Global Arguments SModTr.trans_fnsem: simpl never.
 
-Notation "↧ it" := (SModTr.trans _ _ _ _ _ _ it) (at level 59, only printing).
+Notation "↧ it" := (SModTr.trans _ _ _ it) (at level 59, only printing).
 
 Module SRed. Section RED.
   Context `{!crisG Γ Σ α β τ _S _I, !concG}.
   Import SModTr.
 
   (* reduction lemmas for vis form - used for reduction tactics *)
-  Lemma bind sp msk N stid (R S : Type) (s : itree crisE R) (k : R → itree crisE S) :
-    trans sp msk N stid (s >>= k) =
-    st <- trans sp msk N stid s;; trans sp msk N stid (k st).
+  Lemma bind sp N stid (R S : Type) (s : itree crisE R) (k : R → itree crisE S) :
+    trans sp N stid (s >>= k) =
+    st <- trans sp N stid s;; trans sp N stid (k st).
   Proof using. rewrite /SModTr.trans interpV_bind //. Qed.
 
-  Lemma tau sp msk N stid (U : Type) (t : itree crisE U) :
-    trans sp msk N stid (tau;; t) = tau;; (trans sp msk N stid t).
+  Lemma tau sp N stid (U : Type) (t : itree crisE U) :
+    trans sp N stid (tau;; t) = tau;; (trans sp N stid t).
   Proof using. rewrite /SModTr.trans interpV_tau //. Qed.
 
-  Lemma ret sp msk N stid (U : Type) (t : U) :
-    trans sp msk N stid (Ret t) = Ret t.
+  Lemma ret sp N stid (U : Type) (t : U) :
+    trans sp N stid (Ret t) = Ret t.
   Proof using. rewrite /SModTr.trans interpV_ret //. Qed.
 
-  Lemma vis_agE sp msk N stid {X R} (e : agE X) (ktr : X → itree crisE R) :
-    trans sp msk N stid (vis e ktr) =
-    if msk X (subevent _ e)
-    then vis e (λ x, trans sp msk N stid (ktr x))
-    else vis (Take False) (λ v, Ret (False_rect _ v)).
+  Lemma vis_agE sp N stid {X R} (e : agE X) (ktr : X → itree crisE R) :
+    trans sp N stid (vis e ktr) =
+    vis e (λ x, trans sp N stid (ktr x)).
   Proof using.
-    rewrite /SModTr.trans /SModTr.handle /=; apply observe_eta; rewrite /mask_handle /=.
-    rewrite resum_to_subevent subevent_subevent; des_if; ss; f_equal; extensionality x; grind.
+    rewrite /SModTr.trans /SModTr.handle /=; apply observe_eta; rewrite /=.
+    f_equal; extensionality x; grind.
   Qed.
 
-  Lemma vis_pgE sp msk N stid {X R} (e : pgE X) (ktr : X → itree crisE R) :
-    trans sp msk N stid (vis e ktr) =
-    if msk X (subevent _ e)
-    then vis e (λ x, trans sp msk N stid (ktr x))
-    else vis (Take False) (λ v, Ret (False_rect _ v)).
+  Lemma vis_pgE sp  N stid {X R} (e : pgE X) (ktr : X → itree crisE R) :
+    trans sp  N stid (vis e ktr) =
+    vis e (λ x, trans sp N stid (ktr x)).
   Proof using.
-    rewrite /SModTr.trans /SModTr.handle /=; apply observe_eta; rewrite /mask_handle /=.
-    rewrite !resum_to_subevent !subevent_subevent; des_if; ss; f_equal; extensionality x; grind.
+    rewrite /SModTr.trans /SModTr.handle /=; apply observe_eta; rewrite /=.
+    f_equal; extensionality x; grind.
   Qed.
 
-  Lemma vis_coreE sp msk N stid {X R} (e : coreE X) (ktr : X → itree crisE R) :
-    trans sp msk N stid (vis e ktr) =
-    if msk X (subevent _ e)
-    then vis e (λ x, trans sp msk N stid (ktr x))
-    else vis (Take False) (λ v, Ret (False_rect _ v)).
+  Lemma vis_coreE sp  N stid {X R} (e : coreE X) (ktr : X → itree crisE R) :
+    trans sp  N stid (vis e ktr) =
+    vis e (λ x, trans sp N stid (ktr x)).
   Proof using.
-    rewrite /SModTr.trans /SModTr.handle /=; apply observe_eta; rewrite /mask_handle /=.
-    rewrite !resum_to_subevent !subevent_subevent; des_if; ss; f_equal; extensionality x; grind.
+    rewrite /SModTr.trans /SModTr.handle /=; apply observe_eta; rewrite /=.
+    f_equal; extensionality x; grind.
   Qed.
 
-  Lemma vis_call sp msk N stid {R} fn args (ktr : Any.t → itree crisE R) :
-    trans sp msk N stid (vis (Call fn args) ktr) =
-    tau;; r <- HoareCall msk (sp (speckey_fn fn)) fn args N stid;;
-    trans sp msk N stid (ktr r).
+  Lemma vis_call sp N stid {R} fn args (ktr : Any.t → itree crisE R) :
+    trans sp N stid (vis (Call fn args) ktr) =
+    tau;; r <- HoareCall (sp (speckey_fn fn)) fn args N stid;;
+    trans sp N stid (ktr r).
   Proof using. rewrite /SModTr.trans /SModTr.handle /= interpV_vis. apply observe_eta; ss. Qed.
 
-  Lemma vis_spawn sp msk N stid {R} fn args (ktr : nat → itree crisE R) :
-    trans sp msk N stid (vis (Spawn fn args) ktr) =
-    tau;; r <- HoareSpawn msk (sp (speckey_fn fn)) (sp (speckey_concE)) fn args N;;
-    trans sp msk N stid (ktr r).
+  Lemma vis_spawn sp N stid {R} fn args (ktr : nat → itree crisE R) :
+    trans sp N stid (vis (Spawn fn args) ktr) =
+    tau;; r <- HoareSpawn (sp (speckey_fn fn)) (sp (speckey_concE)) fn args N;;
+    trans sp N stid (ktr r).
   Proof using. rewrite /SModTr.trans /SModTr.handle /= interpV_vis. apply observe_eta; ss. Qed.
 
-  Lemma vis_yield sp msk N stid {R} tid (ktr : () → itree crisE R) :
-    trans sp msk N stid (vis (Yield tid) ktr) =
-    tau;; x <- HoareYield msk (sp (speckey_concE)) N stid tid;; trans sp msk N stid (ktr x).
+  Lemma vis_yield sp N stid {R} tid (ktr : () → itree crisE R) :
+    trans sp N stid (vis (Yield tid) ktr) =
+    tau;; x <- HoareYield (sp (speckey_concE)) N stid tid;; trans sp N stid (ktr x).
   Proof using. rewrite /SModTr.trans /SModTr.handle /= interpV_vis. apply observe_eta; ss. Qed.
 
-  Lemma vis_gettid sp msk N stid {R} (ktr : nat → itree crisE R) :
-    trans sp msk N stid (vis GetTid ktr) =
-    tau;; x <- HoareGetTid msk (sp (speckey_concE)) stid;; trans sp msk N stid (ktr x).
+  Lemma vis_gettid sp N stid {R} (ktr : nat → itree crisE R) :
+    trans sp N stid (vis GetTid ktr) =
+    tau;; x <- HoareGetTid (sp (speckey_concE)) stid;; trans sp N stid (ktr x).
   Proof using. rewrite /SModTr.trans /SModTr.handle /= interpV_vis. apply observe_eta; ss. Qed.
 
-  Lemma assumeK sp msk N stid {R} P (itr : itree crisE R) :
-    trans sp msk N stid (assumeK P itr) =
-    if msk _ (subevent _ (Take P))
-    then assumeK P (trans sp msk N stid itr)
-    else triggerUB.
-  Proof using.
-    apply observe_eta; ss.
-    rewrite resum_to_subevent /mask_handle subevent_subevent.
-    des_if; ss; f_equal; extensionality x; grind.
-  Qed.
+  Lemma assumeK sp N stid {R} P (itr : itree crisE R) :
+    trans sp N stid (assumeK P itr) = assumeK P (trans sp N stid itr).
+  Proof using. apply observe_eta; ss; f_equal; extensionality x; grind. Qed.
 
-  Lemma guaranteeK sp msk N stid {R} P (itr : itree crisE R) :
-    trans sp msk N stid (guaranteeK P itr) =
-    if msk _ (subevent _ (Choose P))
-    then guaranteeK P (trans sp msk N stid itr)
-    else triggerUB.
-  Proof using.
-    apply observe_eta; ss.
-    rewrite resum_to_subevent /mask_handle subevent_subevent.
-    des_if; ss; f_equal; extensionality x; grind.
-  Qed.
+  Lemma guaranteeK sp N stid {R} P (itr : itree crisE R) :
+    trans sp N stid (guaranteeK P itr) = guaranteeK P (trans sp N stid itr).
+  Proof using. apply observe_eta; ss; f_equal; extensionality x; grind. Qed.
 
-  Lemma unwrapUK sp msk N stid {X R} x (ktr : X → itree crisE R) :
-    trans sp msk N stid (unwrapUK x ktr) =
-    unwrapUK x (λ x, trans sp msk N stid (ktr x)).
-  Proof using.
-    destruct x; ss.
-    eapply observe_eta; ss.
-    rewrite /mask_handle resum_to_subevent subevent_subevent.
-    des_if; ss; f_equal; grind; extensionality x; ss.
-  Qed.
+  Lemma unwrapUK sp N stid {X R} x (ktr : X → itree crisE R) :
+    trans sp N stid (unwrapUK x ktr) = unwrapUK x (λ x, trans sp N stid (ktr x)).
+  Proof using. destruct x; ss. eapply observe_eta; ss. f_equal; grind; extensionality x; ss. Qed.
 
-  Lemma unwrapNK sp msk N stid {X R} (x : option X) (ktr : X → itree crisE R) :
-    trans sp msk N stid (unwrapNK x ktr) =
-    if (msk _ (subevent _ (Choose False)))
-    then unwrapNK x (λ x, trans sp msk N stid (ktr x))
-    else Events.unwrapUK x (λ x, trans sp msk N stid (ktr x)).
+  Lemma unwrapNK sp N stid {X R} (x : option X) (ktr : X → itree crisE R) :
+    trans sp N stid (unwrapNK x ktr) = unwrapNK x (λ x, trans sp N stid (ktr x)).
   Proof using.
     destruct x; [des_ifs|]; ss.
-    apply observe_eta; ss.
-    rewrite /mask_handle resum_to_subevent subevent_subevent; des_if; ss.
-    { f_equal; extensionalities x; ss. }
-    { f_equal; extensionalities x; ss. }
+    apply observe_eta; ss; f_equal; extensionality x; ss.
   Qed.
 
   (* reduction lemmas for trigger form *)
-  Lemma yield sp msk N stid tid :
-    trans sp msk N stid (trigger (Yield tid)) =
-    tau;; HoareYield msk (sp (speckey_concE)) N stid tid.
+  Lemma yield sp N stid tid :
+    trans sp N stid (trigger (Yield tid)) =
+    tau;; HoareYield (sp (speckey_concE)) N stid tid.
   Proof using. rewrite vis_yield; grind; erewrite <- bind_ret_r; grind; rewrite ret //. Qed.
 
-  Lemma spawn sp msk N stid fn args :
-    trans sp msk N stid (trigger (Spawn fn args)) =
-    tau;; HoareSpawn msk (sp (speckey_fn fn)) (sp (speckey_concE)) fn args N.
+  Lemma spawn sp N stid fn args :
+    trans sp N stid (trigger (Spawn fn args)) =
+    tau;; HoareSpawn (sp (speckey_fn fn)) (sp (speckey_concE)) fn args N.
   Proof using. rewrite vis_spawn; grind; erewrite <- bind_ret_r; grind; rewrite ret //. Qed.
 
-  Lemma gettid sp msk N stid :
-    trans sp msk N stid (trigger GetTid) = tau;; HoareGetTid msk (sp (speckey_concE)) stid.
+  Lemma gettid sp N stid :
+    trans sp N stid (trigger GetTid) = tau;; HoareGetTid (sp (speckey_concE)) stid.
   Proof using. rewrite vis_gettid; grind; erewrite <- bind_ret_r; grind; rewrite ret //. Qed.
 
-  Lemma call sp msk N stid fn args :
-    trans sp msk N stid (trigger (Call fn args)) =
-    tau;; HoareCall msk (sp (speckey_fn fn)) fn args N stid.
+  Lemma call sp N stid fn args :
+    trans sp N stid (trigger (Call fn args)) =
+    tau;; HoareCall (sp (speckey_fn fn)) fn args N stid.
   Proof using. rewrite vis_call; grind; erewrite <- bind_ret_r; grind; rewrite ret //. Qed.
 
-  Lemma pg sp msk N stid (R : Type) (e : pgE R) :
-    trans sp msk N stid (trigger e) = mask_trigger msk e.
+  Lemma pg sp N stid (R : Type) (e : pgE R) : trans sp N stid (trigger e) = trigger e.
   Proof using.
-    rewrite vis_pgE mask_trigger_gen; des_if; rewrite vis_trigger; grind.
-    erewrite <- bind_ret_r; grind; rewrite ret //.
+    rewrite vis_pgE vis_trigger; grind; erewrite <- bind_ret_r; grind; rewrite ret //.
   Qed.
 
-  Lemma core sp msk N stid (R : Type) (e : coreE R) : 
-    trans sp msk N stid (trigger e) = mask_trigger msk e.
+  Lemma core sp N stid (R : Type) (e : coreE R) :
+    trans sp N stid (trigger e) = trigger e.
   Proof using.
-    rewrite vis_coreE mask_trigger_gen; des_if; rewrite vis_trigger; grind.
-    erewrite <- bind_ret_r; grind; rewrite ret //.
+    rewrite vis_coreE vis_trigger; grind; erewrite <- bind_ret_r; grind; rewrite ret //.
   Qed.
 
-  Lemma ag sp msk N stid (R : Type) (e : agE R) : 
-    trans sp msk N stid (trigger e) = mask_trigger msk e.
+  Lemma ag sp N stid (R : Type) (e : agE R) : trans sp N stid (trigger e) = trigger e.
   Proof using.
-    rewrite vis_agE mask_trigger_gen; des_if; rewrite vis_trigger; grind.
-    erewrite <- bind_ret_r; grind; rewrite ret //.
+    rewrite vis_agE vis_trigger; grind; erewrite <- bind_ret_r; grind; rewrite ret //.
   Qed.
 
   (* Lemma unwrapU (R : Type) (i : option R) :
